Remove most fun parts of expressions

Imp/Expr/Eval.lean
@@ -24,16 +24,15 @@ def get (x : String) (σ : Env) : Value :=
 def init (i : Value) : Env := fun _ => i
 
 @[simp]
-theorem get_init : (Env.init v).get x = v := by rfl
+theorem get_init : (Env.init v).get x = v := by sorry
 
 @[simp]
 theorem get_set_same {σ : Env} : (σ.set x v).get x = v := by
-  simp [get, set]
+  sorry
 
 @[simp]
 theorem get_set_different {σ : Env} : x ≠ y → (σ.set x v).get y = σ.get y := by
-  intros
-  simp [get, set, *]
+  sorry
 
 end Env
 
@@ -66,12 +65,7 @@ Evaluates an expression, finding the value if it has one.
 Expressions that divide by zero don't have values - the result is undefined.
 -/
 def eval (σ : Env) : Expr → Option Value
-  | .const i => some i
-  | .var x => σ.get x
-  | .un op e => do
-    let v ← e.eval σ
-    op.apply v
-  | .bin op e1 e2 => do
-    let v1 ← e1.eval σ
-    let v2 ← e2.eval σ
-    op.apply v1 v2
+  | .const i => sorry
+  | .var x => sorry
+  | .un op e => sorry
+  | .bin op e1 e2 => sorry
