Imp/Expr/Optimize.lean
@@ -7,38 +7,14 @@ namespace Imp.Expr
 Optimizes an expression by folding constants.
 -/
 def optimize : Expr → Expr
-  | .const i => .const i
-  | .var x => .var x
-  | .un op e =>
-    match optimize e with
-    | .const i =>
-      if let some v := op.apply i then .const v
-      else .un op (.const i)
-    | e' => .un op e'
-  | .bin op e1 e2 =>
-    match optimize e1, optimize e2 with
-    | .const i, .const i' =>
-      if let some v := op.apply i i' then .const v
-      else .bin op (.const i) (.const i')
-    | e1', e2' => .bin op e1' e2'
+  | expr => expr
 
 /--
 Optimization doesn't change the meaning of any expression
 -/
-theorem optimize_ok (e : Expr) : e.eval σ = e.optimize.eval σ := by
-  induction e <;> simp [optimize]
-  case un op e ih =>
-    split <;> simp [eval, *]
-    cases op <;> simp [UnOp.apply, eval]
-  case bin op e1 e2 ih1 ih2 =>
-    split <;> simp [eval, *]
-    cases op <;> simp [BinOp.apply, eval]
-    split
-    . simp [eval, BinOp.apply]; split <;> trivial
-    . simp [eval]
+theorem optimize_ok (e : Expr) : e.eval σ = e.optimize.eval σ := by sorry
 
 /--
 Optimization doesn't change the meaning of any expression
 -/
-theorem optimize_ok' (e : Expr) : e.eval σ = e.optimize.eval σ := by
-  induction e using optimize.induct <;> simp [optimize, eval, *]
+theorem optimize_ok' (e : Expr) : e.eval σ = e.optimize.eval σ := by sorry
